theories/logrel/fundamental_prim.v
@@ -3,7 +3,7 @@ From machine_program_logic.program_logic Require Import weakestpre.
 From HypVeri.lang Require Import lang trans_extra.
 From HypVeri.algebra Require Import base pagetable mem trans.
 From HypVeri.rules Require Import rules_base mov yield ldr halt fail add sub mult cmp br bne str run.
-From HypVeri.logrel Require Import logrel_prim.
+From HypVeri.logrel Require Import logrel_prim_extra.
 (* From HypVeri.logrel Require Import ftlr_nop ftlr_run ftlr_yield ftlr_share ftlr_retrieve ftlr_relinquish ftlr_reclaim ftlr_donate ftlr_lend *)
 (*   ftlr_msg_send ftlr_msg_wait ftlr_msg_poll ftlr_invalid_hvc. *)
 From HypVeri Require Import proofmode.
@@ -14,10 +14,110 @@ Section fundamental_prim.
   Context `{hypparams:!HypervisorParameters}.
   Context `{vmG: !gen_VMG Σ}.
 
-  Lemma ftlr_p `{!SliceWf Φ}:
-  ∀ p_tx p_rx ps_acc trans, interp_access_prim Φ p_tx p_rx ps_acc trans ⊢ interp_execute V0.
+  Lemma ftlr_p Φ `(!SliceWf Φ):
+  ∀ p_tx p_rx ps_acc trans, interp_access_prim Φ p_tx p_rx ps_acc trans ⊢ interp_execute_prim.
   Proof.
     rewrite /interp_access_prim /=.
+    iIntros (????) "(%HΦ & (%regs & %Htotal_regs & regs) & (tx & [% mem_tx]) & pgt_acc & %Hsubset_mb & %Hsubset_acc & pgt_owned & tran_pgt_owned &
+                           retri_owned & mem_owned & VMProp & rx_state & rx & [% mem_rx] & trans_hpool_global & other_rx & transferred & VMProps)".
+
+    iDestruct (big_sepSS_difference_singleton _ V0 with "transferred") as "[transferred_except transferred_only]";eauto.
+    apply elem_of_set_of_vmids.
+    iDestruct (get_trans_ps_disj with "trans_hpool_global") as %Htrans_disj.
+    iDestruct (get_trans_neq with "trans_hpool_global") as %Htrans_neq.
+    iDestruct (transferred_only_equiv with "transferred_only") as "(tran_pgt_transferred & retri & mem_transferred)";eauto.
+
+    iDestruct (memory_pages_oea_transferred with "[$mem_owned $mem_transferred]") as (?) "mem";eauto.
+    clear Htrans_disj Htrans_neq.
+
+    set i := V0.
+    set ps_mem_in_trans := (accessible_in_trans_memory_pages i trans).
+
+    iDestruct (memory_pages_disj_singleton with "[$mem $mem_rx]") as %Hnin_rx.
+    iDestruct (memory_pages_disj_singleton with "[$mem $mem_tx]") as %Hnin_tx.
+    (* merge all memory pages together *)
+    iDestruct (memory_pages_merge_mb with "[$mem mem_rx mem_tx]") as "mem";auto.
+    iCombine "mem_tx mem_rx" as "mem". iExact "mem".
+    iDestruct "tx" as "[tx pgt_tx]".
+    clear mem_rx mem_tx mem_all; subst ps_mem_in_trans.
+
+    iLöb as "IH" forall (regs ps_acc trans Htotal_regs Hsubset_mb Hsubset_acc Hnin_rx Hnin_tx).
+    set ps_mem_in_trans := (accessible_in_trans_memory_pages i trans).
+
+    (* split memory pages into [mem_acc] and [mem_rest] *)
+    iDestruct (memory_pages_split_diff' _ ps_acc with "mem") as "[mem_rest mem_acc]". set_solver.
+    iDestruct (memory_pages_split_singleton' p_tx ps_acc with "mem_acc") as "[mem_acc_tx mem_tx]". set_solver + Hsubset_mb.
+    iDestruct ("mem_acc_tx") as (mem_acc_tx) "mem_acc_tx".
+
+    pose proof (Htotal_regs PC) as Hlookup_PC.
+    destruct Hlookup_PC as [ai Hlookup_PC].
+    (* sswp *)
+    rewrite /interp_execute_prim. rewrite ->wp_sswp.
+    destruct (decide ((tpa ai) ∈ ps_acc)) as [Hin_ps_acc | Hnotin_ps_acc].
+    { (* i has access *)
+      destruct (decide (tpa ai = p_tx)) as [Heq_ptx | Hneq_ptx].
+      { (*invalid instruction location *)
+        iDestruct (reg_big_sepM_split i Hlookup_PC with "[$regs]") as "[PC _]".
+        iApply (invalid_pc_in_tx _ ai with "[PC tx]"); iFrameAutoSolve.
+        iNext.
+        iIntros "? _".
+        by iApply wp_terminated.
+      }
+      assert (Hin_ps_acc_tx': (tpa ai) ∈ ps_acc ∖ {[p_tx]}).
+      { set_solver + Hin_ps_acc Hneq_ptx. }
+      iDestruct "mem_acc_tx" as "[%Hdom_mem_acc_tx mem_acc_tx]".
+      pose proof Hin_ps_acc_tx' as Hin_ps_acc_tx.
+      apply elem_of_set_of_addr_tpa in Hin_ps_acc_tx'.
+      rewrite -Hdom_mem_acc_tx in Hin_ps_acc_tx'.
+      rewrite elem_of_dom in Hin_ps_acc_tx'.
+      destruct Hin_ps_acc_tx' as [instr Hlookup_mem_ai].
+      destruct (decode_instruction instr) as [instr'|] eqn:Heqn.
+      { (* valid instruction *)
+        destruct instr'.
+        { admit. }
+        { admit. }
+        { admit. }
+        { admit. }
+        { admit. }
+        { admit. }
+        { admit. }
+        { admit. }
+        { admit. }
+        { admit. }
+        { admit. }
+        { admit. }
+        {
+          pose proof (Htotal_regs R0) as [r0 Hlookup_reg_R0].
+          destruct (decode_hvc_func r0) as [hvc_f |] eqn:Hdecode_hvc .
+          {
+            iAssert (⌜p_tx ≠ p_rx⌝)%I as "%Hneq_mb".
+            {
+              iDestruct "rx" as "[_ [_ excl_rx]]".
+              iDestruct "pgt_tx" as "[_ excl_tx]".
+              iApply (excl_ne with "[$ excl_tx $ excl_rx]").
+            }
+            destruct (hvc_f).
+            { (* RUN *)
+              admit. }
+            { admit. }
+            { admit. }
+            { admit. }
+            { admit. }
+            { admit. }
+            { admit. }
+            { admit. }
+            { (* SEND *)
+              admit. }
+            { (* WAIT *)
+              admit. }
+            { admit. }
+          }
+          admit.
+        }
+      }
+      admit.
+    }
+    admit.
   Admitted.
 
 End fundamental_prim.
